Parameters removed from eta expanded data constructord in L3.  Also TSort, TProd and TInd removed from L3.  Tested but not completely proved.

certicoq/theories/L2_5_box/stripEvalCommute.v
@@ -7,11 +7,10 @@ Require Import Coq.Arith.Peano_dec.
 Require Import Coq.Setoids.Setoid.
 Require Import Omega.
 
-Require Import L2.L2.
+Require Import L2k.L2k.
 Require Import L2_5.compile.
 Require Import L2_5.term.
 Require Import L2_5.program.
-Require Import L2_5.wndEval.
 Require Import L2_5.wcbvEval.
 
 Local Open Scope string_scope.
@@ -19,49 +18,49 @@ Local Open Scope bool.
 Local Open Scope list.
 Set Implicit Arguments.
 
-Definition L2Term := L2.compile.Term.
-Definition L2Terms := L2.compile.Terms.
-Definition L2Defs := L2.compile.Defs.
-Definition strip := L2Term_Term.
-Definition strips := L2Terms_Terms.
-Definition stripDs := L2Defs_Defs.
-Definition stripEnv := L2Env_Env.
-Definition stripEc := L2EC_EC.
+Definition L2kTerm := L2k.compile.Term.
+Definition L2kTerms := L2k.compile.Terms.
+Definition L2kDefs := L2k.compile.Defs.
+Definition strip := L2kTerm_Term.
+Definition strips := L2kTerms_Terms.
+Definition stripDs := L2kDefs_Defs.
+Definition stripEnv := L2kEnv_Env.
+Definition stripEc := L2kEC_EC.
 
 Lemma isApp_strip_TApp:
-  forall s1 s2 s3, isApp (strip (L2.compile.TApp s1 s2 s3)).
+  forall s1 s2 s3, isApp (strip (L2k.compile.TApp s1 s2 s3)).
 Proof.
   intros s1 s2 s3.
   change (isApp (mkApp (strip s1) (tcons (strip s2) (strips s3)))).
   apply (mkApp_isApp (strip s1) (strip s2) (strips s3)).
 Qed.                          
 
-Definition optStrip (t:option L2Term) : option Term :=
+Definition optStrip (t:option L2kTerm) : option Term :=
   match t with
     | None => None
     | Some t => Some (strip t)
   end.
-Definition optL2Terms_Terms (ts:option L2Terms) : option Terms :=
+Definition optL2kTerms_Terms (ts:option L2kTerms) : option Terms :=
   match ts with
     | None => None
-    | Some ts => Some (L2Terms_Terms ts)
+    | Some ts => Some (L2kTerms_Terms ts)
   end.
-Definition optStripDnth (b: option (L2Term * nat)) : option (Term * nat) :=
+Definition optStripDnth (b: option (L2kTerm * nat)) : option (Term * nat) :=
                            match b with
                              | None => None
                              | Some (t, n) => Some (strip t, n)
                            end.
 Definition optStripCanP
-           (b: option (nat * L2Terms * nat)): option (nat * Terms * nat) :=
+           (b: option (nat * L2kTerms * nat)): option (nat * Terms * nat) :=
                            match b with
                              | None => None
-                             | Some (n, t, m) => Some (n, L2Terms_Terms t, m)
+                             | Some (n, t, m) => Some (n, L2kTerms_Terms t, m)
                            end.
 
 Lemma optStrip_hom: forall y, optStrip (Some y) = Some (strip y).
 induction y; simpl; reflexivity.
 Qed.
-Lemma optL2Terms_Terms_hom: forall y, optL2Terms_Terms (Some y) = Some (L2Terms_Terms y).
+Lemma optL2kTerms_Terms_hom: forall y, optL2kTerms_Terms (Some y) = Some (L2kTerms_Terms y).
 induction y; simpl; reflexivity.
 Qed.
 Lemma optStripDnth_hom:
@@ -69,27 +68,27 @@ Lemma optStripDnth_hom:
 induction y; simpl; reflexivity.
 Qed.
 Lemma optStripCanP_hom:
-  forall y n m, optStripCanP (Some (n, y, m)) = Some (n, L2Terms_Terms y, m).
+  forall y n m, optStripCanP (Some (n, y, m)) = Some (n, L2kTerms_Terms y, m).
 induction y; simpl; reflexivity.
 Qed.
                               
 Lemma Lookup_hom:
-  forall (p:environ L2.compile.Term) s ec, Lookup s p ec -> Lookup s (L2Env_Env p) (L2EC_EC ec).
+  forall (p:environ L2k.compile.Term) s ec, Lookup s p ec -> Lookup s (L2kEnv_Env p) (L2kEC_EC ec).
 Proof.
   induction 1; destruct t.
-  - change (Lookup s ((s, ecTrm (strip t)) :: (L2Env_Env p))
+  - change (Lookup s ((s, ecTrm (strip t)) :: (L2kEnv_Env p))
                    (ecTrm (strip t))).
     apply LHit.
   - cbn. apply LHit.
-  - change (Lookup s2 ((s1, ecTrm (strip t)) :: (L2Env_Env p))
-                   (L2EC_EC ec)).
+  - change (Lookup s2 ((s1, ecTrm (strip t)) :: (L2kEnv_Env p))
+                   (L2kEC_EC ec)).
     apply LMiss; assumption.
   - cbn. apply LMiss; assumption.
 Qed.
 
 Lemma lookup_hom:
   forall p nm ec,
-    lookup nm p = Some ec -> lookup nm (stripEnv p) = Some (L2EC_EC ec).
+    lookup nm p = Some ec -> lookup nm (stripEnv p) = Some (L2kEC_EC ec).
 Proof.
   intros p nm ec h. apply Lookup_lookup.
   apply Lookup_hom. apply (lookup_Lookup _ _ h).
@@ -97,7 +96,7 @@ Qed.
   
 Lemma lookup_hom_None:
   forall p nm,
-    lookup nm p = None -> lookup nm (L2Env_Env p) = None.
+    lookup nm p = None -> lookup nm (L2kEnv_Env p) = None.
 Proof.
   induction p; intros.
   - cbn. reflexivity.
@@ -133,33 +132,33 @@ Proof.
 Qed.
 
 Lemma dlength_hom:
-  forall ds, L2.term.dlength ds = dlength (stripDs ds).
+  forall ds, L2k.compile.dlength ds = dlength (stripDs ds).
 induction ds. intuition. simpl. rewrite IHds. reflexivity.
 Qed.
 
 Lemma tcons_hom:
-  forall t ts, L2Terms_Terms (L2.compile.tcons t ts) =
-               tcons (strip t) (L2Terms_Terms ts).
+  forall t ts, L2kTerms_Terms (L2k.compile.tcons t ts) =
+               tcons (strip t) (L2kTerms_Terms ts).
 reflexivity.
 Qed.
 
-Lemma tnil_hom: L2Terms_Terms L2.compile.tnil = tnil.
+Lemma tnil_hom: L2kTerms_Terms L2k.compile.tnil = tnil.
 reflexivity.
 Qed.
 
 Lemma dcons_hom:
   forall nm bod rarg ds,
-    stripDs (L2.compile.dcons nm bod rarg ds) =
+    stripDs (L2k.compile.dcons nm bod rarg ds) =
     dcons nm (strip bod) rarg (stripDs ds).
 reflexivity.
 Qed.
 
-Lemma dnil_hom: stripDs L2.compile.dnil = dnil.
+Lemma dnil_hom: stripDs L2k.compile.dnil = dnil.
 reflexivity.
 Qed.
 
 Lemma dnthBody_hom: 
-  forall m ds, optStripDnth (L2.term.dnthBody m ds) =
+  forall m ds, optStripDnth (L2k.term.dnthBody m ds) =
                dnthBody m (stripDs ds).
 induction m; induction ds; try intuition.
 - simpl. intuition.
@@ -167,23 +166,23 @@ Qed.
 
 Lemma tappend_hom:
   forall ts us,
-    L2Terms_Terms (L2.term.tappend ts us) =
-    tappend (L2Terms_Terms ts) (L2Terms_Terms us).
+    L2kTerms_Terms (L2k.term.tappend ts us) =
+    tappend (L2kTerms_Terms ts) (L2kTerms_Terms us).
 induction ts; intros us; simpl. reflexivity.
 rewrite IHts. reflexivity.
 Qed.
 
 Lemma TCase_hom:
   forall m mch brs,
-    strip (L2.compile.TCase m mch brs) =
-      match L2.term.isProof_dec mch with
+    strip (L2k.compile.TCase m mch brs) =
+      match L2k.term.isProof_dec mch with
         | left _ =>
           match brs with
-            | L2.compile.dunit _ br n =>
-              applyBranchToProof n (L2Term_Term br)
-            | _ => TCase m (L2Term_Term mch) (L2Defs_Defs brs)
+            | L2k.compile.dunit _ br n =>
+              applyBranchToProof n (L2kTerm_Term br)
+            | _ => TCase m (L2kTerm_Term mch) (L2kDefs_Defs brs)
           end
-        | right _ => TCase m (L2Term_Term mch) (L2Defs_Defs brs)
+        | right _ => TCase m (L2kTerm_Term mch) (L2kDefs_Defs brs)
       end.
 Proof.
   reflexivity.
@@ -192,14 +191,14 @@ Qed.
 
 Lemma TApp_hom:
   forall fn arg args,
-    strip (L2.compile.TApp fn arg args) =
-    mkApp (strip fn) (strips (L2.compile.tcons arg args)).
+    strip (L2k.compile.TApp fn arg args) =
+    mkApp (strip fn) (strips (L2k.compile.tcons arg args)).
   induction fn; intros arg args; try reflexivity.
 Qed.
 
 (**
 Lemma hom_isApp:
-  forall t, L2.term.isApp t -> isApp (strip t).
+  forall t, L2k.term.isApp t -> isApp (strip t).
 Proof.
   induction t; cbn; intros; destruct H as [x0 [x1 [x2 jx]]]; try discriminate.
   - myInjection jx. auto.
@@ -209,37 +208,37 @@ Qed.
 Lemma isApp_hom:
   forall t,
     isApp (strip t) ->
-    L2.term.isApp t \/
+    L2k.term.isApp t \/
     exists x n u br nm,
-      t = L2.compile.TCase x (L2.compile.TProof u) (L2.compile.dunit nm br n).
+      t = L2k.compile.TCase x (L2k.compile.TProof u) (L2k.compile.dunit nm br n).
 Proof.
   destruct t; cbn; intros h;
   destruct h as [x0 [x1 [x2 h]]]; try discriminate. 
   - left. exists t1, t2, t3. reflexivity.
   - destruct t; try discriminate. destruct d.
     + discriminate.
-    + right. exists p, n0, t, t0, n. destruct d.
+    + right. exists i, n0, t, t0, n. destruct d.
       * reflexivity.
       * discriminate.
 Qed.
 
 Lemma mkApp_hom:
   forall fn args,
-    strip (L2.term.mkApp fn args) = mkApp (strip fn) (L2Terms_Terms args).
+    strip (L2k.term.mkApp fn args) = mkApp (strip fn) (L2kTerms_Terms args).
 Proof.
-  intros fn args. functional induction (L2.term.mkApp fn args).
+  intros fn args. functional induction (L2k.term.mkApp fn args).
   - rewrite TApp_hom. rewrite TApp_hom. rewrite mkApp_idempotent.
     rewrite tcons_hom. rewrite tcons_hom. rewrite tappend_hom.
     reflexivity.
   - destruct t; try (elim y); try reflexivity.
-    + destruct (L2.term.isProof_dec t).
-      destruct i as [x jx]. subst t.
-      * { destruct (L2.term.is_dunit_dec d).
+    + destruct (L2k.term.isProof_dec t).
+      destruct i0 as [x jx]. subst t.
+      * { destruct (L2k.term.is_dunit_dec d).
           - destruct H as [x0 [x1 [x2 jx]]]. subst d. cbn.
             rewrite mkApp_tnil_ident. reflexivity.
-          - unfold L2Terms_Terms. rewrite mkApp_tnil_ident.
+          - unfold L2kTerms_Terms. rewrite mkApp_tnil_ident.
             reflexivity. }
-      * unfold L2Terms_Terms. rewrite mkApp_tnil_ident.
+      * unfold L2kTerms_Terms. rewrite mkApp_tnil_ident.
         reflexivity.
   - destruct t; try (elim y); try reflexivity.
 Qed.
@@ -292,66 +291,66 @@ Qed.
       
 
 Lemma TCast_hom:
-  forall tm, strip (L2.compile.TCast tm) = TCast (strip tm).
+  forall tm, strip (L2k.compile.TCast tm) = TCast (strip tm).
 Proof.
   reflexivity.
 Qed.
 
 
 Lemma instantiate_hom:
-  (forall bod arg n, strip (L2.term.instantiate arg n bod) =
+  (forall bod arg n, strip (L2k.term.instantiate arg n bod) =
                      instantiate (strip arg) n (strip bod)) /\
-  (forall bods arg n, L2Terms_Terms (L2.term.instantiates arg n bods) =
-                      instantiates (strip arg) n (L2Terms_Terms bods)) /\
-  (forall ds arg n, stripDs (L2.term.instantiateDefs arg n ds) =
+  (forall bods arg n, L2kTerms_Terms (L2k.term.instantiates arg n bods) =
+                      instantiates (strip arg) n (L2kTerms_Terms bods)) /\
+  (forall ds arg n, stripDs (L2k.term.instantiateDefs arg n ds) =
                     instantiateDefs (strip arg) n (stripDs ds)).
 Proof.
 Admitted.
      (**************************
-  apply L2.compile.TrmTrmsDefs_ind; intros; try (simpl; reflexivity).
+  apply L2k.compile.TrmTrmsDefs_ind; intros; try (simpl; reflexivity).
   - simpl. destruct (lt_eq_lt_dec n n0); cbn.
     + destruct s.
       * rewrite (proj1 (nat_compare_gt n0 n)); try omega. cbn. reflexivity.
       * subst n. rewrite (proj2 (nat_compare_eq_iff _ _)); trivial.
-        rewrite L2.term.mkApp_tnil_ident. reflexivity.
+        rewrite L2k.term.mkApp_tnil_ident. reflexivity.
     + rewrite (proj1 (nat_compare_lt n0 n)); trivial.
   - admit.
   - cbn. rewrite H. reflexivity.
   - cbn. rewrite H. reflexivity.
   - cbn. rewrite H. rewrite H0. reflexivity.
-   - change (strip (L2.term.mkApp
-                     (L2.term.instantiate arg n t)
-                     (L2.compile.tcons (L2.term.instantiate arg n t0)
-                                         (L2.term.instantiates arg n t1))) =
-            instantiate (strip arg) n (strip (L2.compile.TApp t t0 t1))). 
+   - change (strip (L2k.term.mkApp
+                     (L2k.term.instantiate arg n t)
+                     (L2k.compile.tcons (L2k.term.instantiate arg n t0)
+                                         (L2k.term.instantiates arg n t1))) =
+            instantiate (strip arg) n (strip (L2k.compile.TApp t t0 t1))). 
 Check TApp_hom. 
     change
-      (strip (L2.term.mkApp
-                (L2.term.instantiate arg n t)
-                (L2.compile.tcons (L2.term.instantiate arg n t0)
-                                   (L2.term.instantiates arg n t1))) =
+      (strip (L2k.term.mkApp
+                (L2k.term.instantiate arg n t)
+                (L2k.compile.tcons (L2k.term.instantiate arg n t0)
+                                   (L2k.term.instantiates arg n t1))) =
        (mkApp (instantiate (strip arg) n (strip t))
               (tcons (instantiate (strip arg) n (strip t0))
-                     (instantiates (strip arg) n (L2Terms_Terms t1))))).
+                     (instantiates (strip arg) n (L2kTerms_Terms t1))))).
     rewrite <- H. rewrite <- H0. rewrite <- H1. 
     Check mkApp_hom. rewrite tcons_hom. reflexivity.
-  - change (TCase p (strip (L2.term.instantiate arg n t0))
-                  (L2Terms_Terms (L2.term.instantiates arg n t1)) =
+  - change (TCase p (strip (L2k.term.instantiate arg n t0))
+                  (L2kTerms_Terms (L2k.term.instantiates arg n t1)) =
             (TCase p (instantiate (strip arg) n (strip t0))
-                   (instantiates (strip arg) n (L2Terms_Terms t1)))).
+                   (instantiates (strip arg) n (L2kTerms_Terms t1)))).
     rewrite H0. rewrite H1. reflexivity.
-  - change (TFix (stripDs (L2.term.instantiateDefs
-                             arg (n0 + L2.compile.dlength d) d)) n =
+  - change (TFix (stripDs (L2k.term.instantiateDefs
+                             arg (n0 + L2k.compile.dlength d) d)) n =
             (TFix (instantiateDefs
                      (strip arg) (n0 + dlength (stripDs d)) (stripDs d)) n)).
     rewrite H. rewrite dlength_hom. reflexivity.
-  - change (tcons (strip (L2.term.instantiate arg n t))
-                  (L2Terms_Terms (L2.term.instantiates arg n t0)) =
+  - change (tcons (strip (L2k.term.instantiate arg n t))
+                  (L2kTerms_Terms (L2k.term.instantiates arg n t0)) =
             tcons (instantiate (strip arg) n (strip t))
-                  (instantiates (strip arg) n (L2Terms_Terms t0))).
+                  (instantiates (strip arg) n (L2kTerms_Terms t0))).
     rewrite H. rewrite H0. reflexivity.
-  - change (dcons n (strip (L2.term.instantiate arg n1 t0)) n0
-                  (stripDs (L2.term.instantiateDefs arg n1 d)) =
+  - change (dcons n (strip (L2k.term.instantiate arg n1 t0)) n0
+                  (stripDs (L2k.term.instantiateDefs arg n1 d)) =
             dcons n (instantiate (strip arg) n1 (strip t0)) n0
                   (instantiateDefs (strip arg) n1 (stripDs d))).
     rewrite H0. rewrite H1. reflexivity.
@@ -360,7 +359,7 @@ Qed.
 
 
 Lemma TProof_strip_inv:
-  forall t, TProof = strip t -> (L2.term.isProof t) \/ (L2.term.isCase t).
+  forall t, TProof = strip t -> (L2k.term.isProof t) \/ (L2k.term.isCase t).
 Proof.
   intros t ht. destruct t; try discriminate.
   - left. exists t. reflexivity.
@@ -368,47 +367,47 @@ Proof.
     destruct t1; cbn in ht; try discriminate.
     + pose proof
            (mkApp_isApp
-              (mkApp (L2Term_Term t1_1)
-                     (tcons (L2Term_Term t1_2) (L2Terms_Terms t)))
-              (L2Term_Term t2) (L2Terms_Terms t3)).
+              (mkApp (L2kTerm_Term t1_1)
+                     (tcons (L2kTerm_Term t1_2) (L2kTerms_Terms t)))
+              (L2kTerm_Term t2) (L2kTerms_Terms t3)).
       destruct H as [x0 [x1 [x2 j]]]. rewrite j in ht. discriminate.
-    + destruct (L2.term.isProof_dec t1).
+    + destruct (L2k.term.isProof_dec t1).
       * destruct
           (mkApp_isApp
              (match d with
-                | L2.compile.dnil => TCase p (L2Term_Term t1) (L2Defs_Defs d)
-                | L2.compile.dunit _ br n =>
-                  applyBranchToProof n (L2Term_Term br)
-                | L2.compile.dcons _ br n (L2.compile.dcons _ _ _ _) =>
-                  TCase p (L2Term_Term t1) (L2Defs_Defs d)
-              end) (L2Term_Term t2) (L2Terms_Terms t3)) as [x0 [x1 [x2 jx]]].
+                | L2k.compile.dnil => TCase i (L2kTerm_Term t1) (L2kDefs_Defs d)
+                | L2k.compile.dunit _ br n =>
+                  applyBranchToProof n (L2kTerm_Term br)
+                | L2k.compile.dcons _ br n (L2k.compile.dcons _ _ _ _) =>
+                  TCase i (L2kTerm_Term t1) (L2kDefs_Defs d)
+              end) (L2kTerm_Term t2) (L2kTerms_Terms t3)) as [x0 [x1 [x2 jx]]].
         rewrite jx in ht. discriminate.
-      * destruct (mkApp_isApp (TCase p (L2Term_Term t1) (L2Defs_Defs d))
-                              (L2Term_Term t2) (L2Terms_Terms t3))
+      * destruct (mkApp_isApp (TCase i (L2kTerm_Term t1) (L2kDefs_Defs d))
+                              (L2kTerm_Term t2) (L2kTerms_Terms t3))
           as [x0 [x1 [x2 jx]]].
         rewrite jx in ht. discriminate.
-  - right. exists p, t, d. reflexivity.
+  - right. exists i, t, d. reflexivity.
 Qed.
 
 Lemma Const_strip_inv:
   forall nm s, TConst nm = strip s ->
-               (L2.compile.TConst nm = s) \/ (L2.term.isCase s).
+               (L2k.compile.TConst nm = s) \/ (L2k.term.isCase s).
 Proof.
   intros nm. destruct s; intros h; try discriminate.
   - left.
-    change (TConst nm = mkApp (L2Term_Term s1)
-                        (tcons (L2Term_Term s2) (L2Terms_Terms t))) in h.
-    pose proof (mkApp_isApp (L2Term_Term s1)
-                            (L2Term_Term s2) (L2Terms_Terms t)) as k.
+    change (TConst nm = mkApp (L2kTerm_Term s1)
+                        (tcons (L2kTerm_Term s2) (L2kTerms_Terms t))) in h.
+    pose proof (mkApp_isApp (L2kTerm_Term s1)
+                            (L2kTerm_Term s2) (L2kTerms_Terms t)) as k.
     destruct k as [x0 [x1 [x2 jx]]]. rewrite jx in h. discriminate.
   - left. cbn in h. myInjection h. reflexivity.
-  - right. exists p, s, d. reflexivity.    
+  - right. exists i, s, d. reflexivity.    
 Qed.
 
 (*************
 Lemma Cast_strip_inv:
   forall tm s, TCast tm = strip s ->
-   exists stm, (L2.compile.TCast stm) = s /\ tm = strip stm.
+   exists stm, (L2k.compile.TCast stm) = s /\ tm = strip stm.
 Proof.
   intros tm; destruct s; intros h; try discriminate.
   - myInjection h. exists s. intuition.
@@ -423,7 +422,7 @@ Qed.
 (*****  HERE
 Lemma Fix_strip_inv:
   forall ds n s, TFix ds n = strip s ->
-    exists sds, (L2.compile.TFix sds n) = s /\ ds = stripDs sds.
+    exists sds, (L2k.compile.TFix sds n) = s /\ ds = stripDs sds.
 Proof.
   intros ds n. destruct s; simpl; intros h; try discriminate.
   - myInjection h. exists d. intuition.
@@ -432,7 +431,7 @@ Qed.
 Lemma App_strip_inv:
   forall fn arg args s, TApp fn arg args = strip s ->
     exists sfn sarg sargs,
-      (L2.compile.TApp sfn sarg sargs) = s /\
+      (L2k.compile.TApp sfn sarg sargs) = s /\
       fn = strip sfn /\ arg = strip sarg /\ args = strips sargs.
 Proof.
   intros fn arg args. destruct s; simpl; intros h; try discriminate.
@@ -442,7 +441,7 @@ Qed.
 Lemma LetIn_strip_inv:
   forall nm dfn bod s, TLetIn nm dfn bod = strip s ->
     exists sdfn sty sbod,
-      (L2.compile.TLetIn nm sdfn sty sbod = s) /\
+      (L2k.compile.TLetIn nm sdfn sty sbod = s) /\
       dfn = strip sdfn /\ bod = strip sbod.
 Proof.
   intros nm dfn bod s. destruct s; simpl; intros h; try discriminate.
@@ -451,7 +450,7 @@ Qed.
 
 Lemma Case_strip_inv:
   forall m mch brs s, TCase m mch brs = strip s ->
-    exists sty smch sbrs, (L2.compile.TCase m sty smch sbrs = s) /\
+    exists sty smch sbrs, (L2k.compile.TCase m sty smch sbrs = s) /\
               mch = strip smch /\ brs = stripDs sbrs.
 Proof.
   intros m mch brs s. destruct s; simpl; intros h; try discriminate.
@@ -459,7 +458,7 @@ Proof.
 Qed.
 
 Lemma tnil_strip_inv:
-  forall ts, tnil = strips ts -> ts = L2.compile.tnil.
+  forall ts, tnil = strips ts -> ts = L2k.compile.tnil.
 Proof.
   induction ts; intros; try reflexivity.
   - simpl in H. discriminate.
@@ -467,7 +466,7 @@ Qed.
 
 Lemma tcons_strip_inv:
   forall t ts us, tcons t ts = strips us ->
-    exists st sts, (L2.compile.tcons st sts = us) /\ 
+    exists st sts, (L2k.compile.tcons st sts = us) /\ 
                    t = strip st /\ ts = strips sts.
 Proof.
   intros t ts us. destruct us; simpl; intros h; try discriminate.
@@ -476,7 +475,7 @@ Qed.
 
 Lemma dcons_strip_inv:
   forall nm t m ts us, dcons nm t m ts = stripDs us ->
-    exists ty st sts, (L2.compile.dcons nm ty st m sts = us) /\ 
+    exists ty st sts, (L2k.compile.dcons nm ty st m sts = us) /\ 
                    t = strip st /\ ts = stripDs sts.
 Proof.
   intros nm t m ts us. destruct us; simpl; intros h; try discriminate.
@@ -487,13 +486,13 @@ Qed.
 
 Lemma WcbvEval_hom:
   forall p,
-    (forall t t', L2.wcbvEval.WcbvEval p t t' ->
+    (forall t t', L2k.wcbvEval.WcbvEval p t t' ->
                   WcbvEval (stripEnv p) (strip t) (strip t')) /\
-    (forall ts ts', L2.wcbvEval.WcbvEvals p ts ts' ->
-                    WcbvEvals (stripEnv p) (L2Terms_Terms ts) (strips ts')).
+    (forall ts ts', L2k.wcbvEval.WcbvEvals p ts ts' ->
+                    WcbvEvals (stripEnv p) (L2kTerms_Terms ts) (strips ts')).
 Proof.
   intros p.
-  apply L2.wcbvEval.WcbvEvalEvals_ind; intros;
+  apply L2k.wcbvEval.WcbvEvalEvals_ind; intros;
   try (solve[constructor; intuition]); try (solve[right; cbn; constructor]).
   - cbn. destruct (strip s); inversion_Clear H.
 
@@ -504,18 +503,18 @@ Proof.
 (***********************)
 Lemma WcbvEval_hom:
   forall p,
-    (forall t t', L2.wcbvEval.WcbvEval p t t' ->
+    (forall t t', L2k.wcbvEval.WcbvEval p t t' ->
                   strip t' = TProof \/
                   WcbvEval (stripEnv p) (strip t) (strip t')) /\
-    (forall ts ts', L2.wcbvEval.WcbvEvals p ts ts' ->
-                    WcbvEvals (stripEnv p) (L2Terms_Terms ts) (strips ts')).
+    (forall ts ts', L2k.wcbvEval.WcbvEvals p ts ts' ->
+                    WcbvEvals (stripEnv p) (L2kTerms_Terms ts) (strips ts')).
 Proof.
   intros p.
-  apply L2.wcbvEval.WcbvEvalEvals_ind; intros;
+  apply L2k.wcbvEval.WcbvEvalEvals_ind; intros;
   try (solve[constructor; intuition]); try (solve[right; cbn; constructor]).
   - intuition. right. cbn. constructor. assumption.
   - destruct H; intuition. cbn.
-    destruct (L2.term.isProof_dec t). cbn.
+    destruct (L2k.term.isProof_dec t). cbn.
     + destruct i. subst t. cbn in H. intuition.
     + destruct t; cbn in H. inversion_Clear w.  inversion_Clear w.
 cbn in H
@@ -531,7 +530,7 @@ cbn in H
   - cbn. econstructor; try eassumption.
     eapply (lookupDfn_hom). assumption.
 (*************
-  - destruct (L2.term.isApp_dec t).
+  - destruct (L2k.term.isApp_dec t).
     + destruct i as [x0 [x1 [x2 jx]]]. subst t. 
       cbn. econstructor. eapply H. intros h. discriminate.
     + cbn. destruct t; cbn; try (solve[eapply H; intros k; discriminate]).
