certicoq/theories/L2k_noCnstrParams/compile.v
@@ -1,0 +1,426 @@
+
+Require Import Coq.Lists.List.
+Require Import Coq.Strings.String.
+Require Import Coq.Arith.Compare_dec.
+Require Import Coq.Arith.Peano_dec.
+Require Import Common.Common.
+Require Import Omega.
+Require Import L2.compile.
+Require Import L2.term.
+
+Local Open Scope string_scope.
+Local Open Scope bool.
+Local Open Scope list.
+Set Implicit Arguments.
+
+Definition L2Term := L2.compile.Term.
+Definition L2Terms := L2.compile.Terms.
+Definition L2Defs := L2.compile.Defs.
+Definition L2Pgm := Program L2Term.
+Definition L2EC := envClass L2Term.
+Definition L2Env := environ L2Term.
+
+
+Inductive Term : Type :=
+| TRel       : nat -> Term
+| TProof     : Term -> Term
+| TCast      : Term -> Term
+| TLambda    : name -> Term -> Term
+| TLetIn     : name -> Term -> Term -> Term
+| TApp       : Term -> Term (* first arg must exist *) -> Terms -> Term
+| TConst     : string -> Term
+| TAx        : Term
+(* constructors fully applied: eta expand and drop parameters *)
+| TConstruct : inductive -> nat (* index *) -> Terms -> Term
+         (* use Defs to code branches in Case *)
+| TCase      : inductive -> Term (* discriminee *) ->
+               Defs (* # args, branch *) -> Term
+| TFix       : Defs -> nat -> Term
+| TWrong     : Term
+with Terms : Type :=
+| tnil : Terms
+| tcons : Term -> Terms -> Terms
+with Defs : Type :=
+| dnil : Defs
+| dcons : name -> Term -> nat -> Defs -> Defs.
+Hint Constructors Term Terms Defs.
+Scheme Trm_ind' := Induction for Term Sort Prop
+  with Trms_ind' := Induction for Terms Sort Prop
+  with Defs_ind' := Induction for Defs Sort Prop.
+Combined Scheme TrmTrmsDefs_ind from Trm_ind', Trms_ind', Defs_ind'.
+Combined Scheme TrmTrms_ind from Trm_ind', Trms_ind'.
+Notation prop := (TSort SProp).
+Notation set_ := (TSort SSet).
+Notation type_ := (TSort SType).
+Notation tunit t := (tcons t tnil).
+Notation dunit nm t m := (dcons nm t m dnil).
+
+Fixpoint Terms_list (ts:Terms) : list Term :=
+  match ts with
+    | tnil => nil
+    | tcons u us => cons u (Terms_list us)
+  end.
+
+Function tlength (ts:Terms) : nat :=
+  match ts with 
+    | tnil => 0
+    | tcons _ ts => S (tlength ts)
+  end.
+
+Lemma tlength_S:
+  forall ts p,
+    tlength ts > p ->
+    exists u us, ts = tcons u us /\ tlength us >= p.
+Proof.
+  induction ts; intros.
+  - cbn in H. omega.
+  - cbn in H. case_eq ts; intros; subst.
+    + exists t, tnil. auto. cbn in H. assert (j:p = 0). omega. subst.
+      intuition.
+    + exists t, (tcons t0 t1). intuition.
+Qed.
+
+Fixpoint tappend (ts1 ts2:Terms) : Terms :=
+  match ts1 with
+    | tnil => ts2
+    | tcons t ts => tcons t (tappend ts ts2)
+  end.
+
+Lemma tappend_tnil: forall ts:Terms, tappend ts tnil = ts.
+Proof.
+  induction ts; simpl; try reflexivity.
+  rewrite IHts. reflexivity.
+Qed.
+
+Lemma tappend_assoc:
+  forall xts yts zts,
+       (tappend xts (tappend yts zts)) = (tappend (tappend xts yts) zts).
+  induction xts; intros yts zts; simpl.
+  - reflexivity.
+  - rewrite IHxts. reflexivity.
+Qed.
+
+Lemma tappend_pres_tlength:
+  forall ts us, tlength (tappend ts us) = (tlength ts) + (tlength us).
+Proof.
+  induction ts; intros.
+  - reflexivity.
+  - cbn. rewrite IHts. reflexivity.
+Qed.
+
+(** reversing Terms **)
+Fixpoint treverse (ts: Terms) : Terms :=
+  match ts with
+    | tnil => tnil
+    | tcons b bs => tappend (treverse bs) (tunit b)
+  end.
+
+Lemma treverse_tappend_distr:
+  forall x y:Terms,
+    treverse (tappend x y) = tappend (treverse y) (treverse x).
+Proof.
+  induction x as [| a l IHl]; cbn; intros.
+  - destruct y as [| a l]; cbn. reflexivity.
+    rewrite tappend_tnil. reflexivity.
+  - rewrite (IHl y). rewrite tappend_assoc. reflexivity.
+Qed.
+
+Remark treverse_tunit:
+  forall (l:Terms) (a:Term),
+    treverse (tappend l (tunit a)) = tcons a (treverse l).
+Proof.
+  intros.
+  apply (treverse_tappend_distr l (tunit a)); simpl; auto.
+Qed.
+
+Lemma treverse_involutive:
+  forall ts:Terms, treverse (treverse ts) = ts.
+Proof.
+  induction ts as [| a l IHl]; cbn; intros. reflexivity.
+  - rewrite treverse_tunit. rewrite IHl. reflexivity.
+Qed.
+   
+Remark tunit_treverse:
+    forall (l:Terms) (a:Term),
+    tappend (treverse l) (tunit a) = treverse (tcons a l).
+Proof.
+  intros. cbn. reflexivity.
+Qed.
+
+Lemma treverse_pres_tlength:
+  forall ts, tlength ts = tlength (treverse ts).
+Proof.
+  induction ts; intros. reflexivity.
+  - cbn. rewrite IHts. rewrite tappend_pres_tlength. cbn. omega.
+Qed.
+  
+Fixpoint dlength (ts:Defs) : nat :=
+  match ts with 
+    | dnil => 0
+    | dcons _ _ _ ts => S (dlength ts)
+  end.
+
+
+(** lift a Term over a new binding **)
+Function lift (n:nat) (t:Term) : Term :=
+  match t with
+    | TRel m => TRel (match m ?= n with
+                        | Lt => m
+                        | _ => S m
+                      end)
+    | TLambda nm bod => TLambda nm (lift (S n) bod)
+    | TLetIn nm df bod => TLetIn nm (lift n df) (lift (S n) bod)
+    | TApp fn arg args => TApp (lift n fn) (lift n arg) (lifts n args)
+    | TConstruct i x args => TConstruct i x (lifts n args)
+    | TCase iparsapb mch brs => TCase iparsapb (lift n mch) (liftDs n brs)
+    | TFix ds y => TFix (liftDs (n + dlength ds) ds) y
+    | _ => t
+  end
+with lifts (n:nat) (ts:Terms) : Terms :=
+       match ts with
+         | tnil => tnil
+         | tcons u us => tcons (lift n u) (lifts n us)
+       end
+with liftDs n (ds:Defs) : Defs :=
+       match ds with
+         | dnil => dnil
+         | dcons nm u j es => dcons nm (lift n u) j (liftDs n es)
+       end.
+Functional Scheme lift_ind' := Induction for lift Sort Prop
+with lifts_ind' := Induction for lifts Sort Prop
+with liftDs_ind' := Induction for liftDs Sort Prop.
+Combined Scheme liftLiftsLiftDs_ind from lift_ind', lifts_ind', liftDs_ind'.
+
+
+Lemma lifts_pres_tlength:
+  forall n ts, tlength (lifts n ts) = tlength ts.
+Proof.
+  induction ts.
+  + reflexivity.
+  + simpl. intuition.
+Qed.
+
+Lemma liftDs_pres_dlength:
+  forall n ds, dlength (liftDs n ds) = dlength ds.
+Proof.
+  induction ds.
+  + reflexivity.
+  + simpl. intuition.
+Qed.
+
+Lemma tappend_pres_lifts:
+  forall ts ss n, lifts n (tappend ts ss) = tappend (lifts n ts) (lifts n ss).
+Proof.
+  induction ts; intros.
+  - reflexivity.
+  - cbn. rewrite IHts. reflexivity.
+Qed.
+  
+Lemma treverse_pres_lifts:
+  forall ts n, lifts n (treverse ts) = treverse (lifts n ts).
+Proof.
+  induction ts; intros.
+  - reflexivity.
+  - cbn. rewrite <- IHts. rewrite tappend_pres_lifts.
+    reflexivity.
+Qed.
+
+
+(** turn (Construct [x1;...;xn; 0;...k-1]])  with arity n+k into
+*** (Lam ... (Lam (Construct [x1;...;xn; 0;...k-1])...))
+*** lift [x1;...;xn] k times,
+*** then append the k fresh variables and surround with k lambdas
+**)
+Function addDummyArgs n args :=
+  match n with
+    | 0 => treverse args
+    | S m => addDummyArgs m (tcons (TRel 0) (lifts 0 args))
+  end.
+         
+Function mkEtaArgs npars nargs args: Terms :=
+  match npars, args with
+    | S m, tcons u us => mkEtaArgs m nargs us
+    | 0, us => (* removed all params, possibly some args left *)
+      (addDummyArgs (nargs - tlength us) (treverse us))
+    | _, tnil => (* possibly some params left, no args visible *)
+      (addDummyArgs nargs tnil)
+  end.
+                                               
+Lemma addDummyArgs_sanity:
+  forall n args, tlength (addDummyArgs n args) = n + (tlength args).
+Proof.
+  induction n; induction args; cbn in *; intros; try reflexivity.
+  - rewrite tunit_treverse. rewrite <- treverse_pres_tlength. reflexivity.
+  - rewrite IHn. cbn. omega.
+  - rewrite IHn. cbn. rewrite lifts_pres_tlength. omega.
+Qed.                                           
+
+(****
+Lemma mkEtaArgs_sanity:
+  forall nargs args npars,
+    (npars <= tlength args) ->
+    tlength (mkEtaArgs npars nargs args) = nargs.
+Proof.
+  induction nargs; induction args; induction npars; cbn in *;
+  intros; try omega.
+  - rewrite treverse_tunit. rewrite treverse_involutive.
+    specialize (IHargs 0). destruct args. cbn in *.
+  - rewrite treverse_tappend_distr. rewrite treverse_involutive.
+    cbn in *. unfold mkEtaArgs in IHargs.
+    admit.
+  - omega.
+  -
+    rewrite treverse_tappend_distr. cbn in *. rewrite treverse_involutive in *.
+
+    + cbn. induction npars.
+      * reflexivity.
+      * cbn in *.
+*************)
+
+  
+(** If there are extra args (more than arity, which cannot happen in
+*** a program checked by Coq) we just truncate them,
+*** and no eta expansion is required 
+**)
+Function mkEtaLams (xtraArity:nat) (body:Term) : Term :=
+  match xtraArity with
+    | 0 => body
+    | S n => TLambda nAnon (mkEtaLams n body)
+  end.
+  
+Function etaExp_cnstr
+           (i:inductive) (x npars nargs:nat) (args:Terms) : Term :=
+  let body := TConstruct i x (mkEtaArgs npars nargs args) in
+  mkEtaLams (npars + nargs - (tlength args)) body.
+
+(****
+Definition etaExp_cnstr
+           (i:inductive) (x npars nargs:nat) (args:Terms) : Term :=
+  let body := TConstruct i x (mkEtaArgs npars nargs args) in
+  match nat_compare npars (tlength args) with
+    | Datatypes.Eq => mkEtaLams nargs body
+    | Gt => mkEtaLams (npars + nargs - (tlength args)) body
+    | Lt => mkEtaLams (npars + nargs - (tlength args)) body
+  end.
+****)
+
+Eval cbn in (etaExp_cnstr (mkInd "" 0) 9 1 2 tnil).
+Eval cbn in (etaExp_cnstr (mkInd "" 0) 9 1 2 (tcons (TConst "A") tnil)).
+Eval cbn in (etaExp_cnstr (mkInd "" 0) 9 1 2
+                          (tcons (TConst "A") (tcons (TConst "b") tnil))).
+Eval cbn in (etaExp_cnstr
+               (mkInd "" 0) 9 1 2
+               (tcons (TConst "A")
+                      (tcons (TConst "b") (tcons (TConst "bs") tnil)))).
+             
+Function strip (t:L2Term) : Term :=
+  match t with
+    | L2.compile.TRel n => TRel n
+    | L2.compile.TSort s => TAx
+    | L2.compile.TProof t => TProof (strip t)
+    | L2.compile.TCast t => TCast (strip t)
+    | L2.compile.TProd nm bod => TAx
+    | L2.compile.TLambda nm bod => TLambda nm (strip bod)
+    | L2.compile.TLetIn nm dfn bod => TLetIn nm (strip dfn) (strip bod)
+    | L2.compile.TApp fn arg args =>
+      let sarg := strip arg in
+      let sargs := strips args in
+      match fn with
+        | L2.compile.TConstruct i m npars nargs =>
+          etaExp_cnstr i m npars nargs (tcons sarg sargs)
+        | _ => TApp (strip fn) sarg sargs
+      end
+    | L2.compile.TConst nm => TConst nm
+    | L2.compile.TAx => TAx
+    | L2.compile.TInd i => TAx
+    | L2.compile.TConstruct i m npars nargs =>
+      etaExp_cnstr i m npars nargs tnil
+    | L2.compile.TCase (i,_) mch brs => TCase i (strip mch) (stripDs brs)
+    | L2.compile.TFix ds n => TFix (stripDs ds) n
+    | L2.compile.TWrong => TWrong
+  end
+with strips (ts:L2Terms) : Terms := 
+  match ts with
+    | L2.compile.tnil => tnil
+    | L2.compile.tcons t ts => tcons (strip t) (strips ts)
+  end
+with stripDs (ts:L2Defs) : Defs := 
+  match ts with
+    | L2.compile.dnil => dnil
+    | L2.compile.dcons nm t m ds => dcons nm (strip t) m (stripDs ds)
+  end.
+
+(****
+Lemma TLambda_strip_inv:
+  forall nm bod t, TLambda nm bod = strip t ->
+                   exists bod', t = L2.compile.TLambda nm bod'.
+Proof.
+  destruct t; intros; cbn in *; try discriminate.
+  - myInjection H. exists t. reflexivity.
+  - destruct t1; try discriminate.
+  -
+Qed.
+*****)  
+
+Lemma strip_pres_dlength:
+  forall ds:L2Defs, L2.term.dlength ds = dlength (stripDs ds).
+Proof.
+  induction ds; intros.
+  - reflexivity.
+  - cbn. rewrite IHds. reflexivity.
+Qed.
+                  
+Lemma strips_pres_tlength:
+  forall ts:L2Terms, L2.term.tlength ts = tlength (strips ts).
+Proof.
+  induction ts; intros.
+  - reflexivity.
+  - cbn. rewrite IHts. reflexivity.
+Qed.
+                  
+  
+(** environments and programs **)
+Function stripEC (ec:L2EC) : AstCommon.envClass Term :=
+  match ec with
+    | ecTrm t => ecTrm (strip t)
+    | ecTyp _ n itp => ecTyp Term n itp
+  end.
+
+Definition  stripEnv : L2Env -> AstCommon.environ Term :=
+  List.map (fun nmec : string * L2EC => (fst nmec, stripEC (snd nmec))).
+
+Lemma stripEcTrm_hom:
+  forall t, stripEC (ecTrm t) = ecTrm (strip t).
+Proof.
+  intros. reflexivity.
+Qed.
+
+Lemma stripEnv_pres_fresh:
+  forall nm p, fresh nm p -> fresh nm (stripEnv p).
+Proof.
+  induction 1.
+  - constructor; assumption.
+  - constructor.
+Qed.
+
+Lemma stripEnv_inv:
+  forall gp s ec p, stripEnv gp = (s, ec) :: p ->
+                    exists ec2 p2, ec =stripEC ec2 /\ p = stripEnv p2.
+Proof.
+  intros. destruct gp. discriminate. cbn in H. injection H; intros. subst.
+  exists (snd p0), gp. intuition.
+Qed.
+
+
+Definition stripProgram (p:L2Pgm) : Program Term :=
+  {| env:= stripEnv (env p);
+     main:= strip (main p) |}.
+
+(*** from L1g to L2k ***)
+Definition program_Program (p:program) : Program Term :=
+  stripProgram (L2.compile.program_Program p).
+
+(***
+Definition term_Term (e:AstCommon.environ L1g.compile.Term) (t:term) : Term :=
+  strip (L2.compile.term_Term e t).
+***)
