certicoq/theories/L3_flattenedApp/L3.v
@@ -1,5 +1,5 @@
 (** Collect all of L3 together **)
 
 Require Export L3.compile.
-Require Export L3.term L3.program L3.wndEval L3.wcbvEval L3.wNorm 
+Require Export L3.term L3.program L3.wcbvEval L3.wNorm 
         L3.unaryApplications.
